Prove Ladder and PointCompress, assuming correctness of bignum

code/experimental/ed25519/Hacl.Impl.Ed25519.Field56.fst
@@ -15,73 +15,8 @@ open FStar.Calc
 
 let felem = lbuffer uint64 5ul
 
-let point = lbuffer uint64 20ul
-
-let paren_mul4 (a b c d:nat) : Lemma (a * b * c * d == a * (b * c * d))
-  = ()
-
-let paren_mul5 (a b c d e:nat) : Lemma (a * b * c * d * e == a * (b * c * d * e))
-  = ()
-
-
-#set-options "--z3rlimit 20 --max_fuel 0 --max_ifuel 0"
-
-let lemma_fits_as_nat5 (f:S.felem5) : Lemma (S.as_nat5 f < pow2 256) =
-  let (s0, s1, s2, s3, s4) = f in
-  let max0 = pow2 56 - 1 in
-  let max1 = (pow2 56 - 1) * pow2 56 in
-  let max2 = (pow2 56 - 1) * pow2 56 * pow2 56 in
-  let max3 = (pow2 56 - 1) * pow2 56 * pow2 56 * pow2 56 in
-  let max4 = (pow2 32 - 1) * pow2 56 * pow2 56 * pow2 56 * pow2 56 in
-  let x0 = uint_v s0 % S.pow56 in
-  let x1 = (uint_v s1 % S.pow56) * S.pow56 in
-  let x2 = (uint_v s2 % S.pow56) * S.pow56 * S.pow56 in
-  let x3 = (uint_v s3 % S.pow56) * S.pow56 * S.pow56 * S.pow56 in
-  let x4 = (uint_v s4 % S.pow32) * S.pow56 * S.pow56 * S.pow56 * S.pow56 in
-
-  calc ( <= ) {
-    x1;
-    ( <= ) { FStar.Math.Lemmas.lemma_mult_le_right S.pow56 (uint_v s1 % S.pow56) (pow2 56 - 1) }
-    max1;
-  };
-
-  calc ( <= ) {
-    x2;
-    (==) { FStar.Math.Lemmas.paren_mul_right (uint_v s2 % S.pow56) S.pow56 S.pow56 }
-    (uint_v s2 % S.pow56)  * (S.pow56 * S.pow56);
-    ( <= ) { FStar.Math.Lemmas.lemma_mult_le_right (S.pow56 * S.pow56) (uint_v s2 % S.pow56) (pow2 56 - 1) }
-    max2;
-  };
-  calc ( <= ) {
-    x3;
-    (==) { paren_mul4 (uint_v s3 % S.pow56) S.pow56 S.pow56 S.pow56 }
-    (uint_v s3 % S.pow56) * (S.pow56 * S.pow56 * S.pow56);
-    ( <= ) { FStar.Math.Lemmas.lemma_mult_le_right
-            (S.pow56 * S.pow56 * S.pow56)
-            (uint_v s3 % S.pow56)
-            (pow2 56 - 1) }
-    (pow2 56 - 1) * (S.pow56 * S.pow56 * S.pow56);
-    (==) { paren_mul4 (pow2 56 - 1)  S.pow56 S.pow56 S.pow56 }
-    max3;
-  };
-  calc ( <= ) {
-    x4;
-    (==) { paren_mul5 (uint_v s4 % S.pow32) S.pow56 S.pow56 S.pow56 S.pow56 }
-    (uint_v s4 % S.pow32)  * (S.pow56 * S.pow56 * S.pow56 * S.pow56);
-    ( <= ) { FStar.Math.Lemmas.lemma_mult_le_right
-            (S.pow56 * S.pow56 * S.pow56 * S.pow56)
-            (uint_v s4 % S.pow32)
-            (pow2 32 - 1) }
-    (pow2 32 - 1) * (S.pow56 * S.pow56 * S.pow56 * S.pow56);
-    (==) { paren_mul5 (pow2 32 - 1) S.pow56 S.pow56 S.pow56 S.pow56 }
-    max4;
-  };
-
-  let max = max0 + max1 + max2 + max3 + max4 in
-  assert_norm (max < pow2 256)
-
 noextract
-val as_nat: h:mem -> e:felem -> GTot (n:nat{n < pow2 256})
+val as_nat: h:mem -> e:felem -> GTot nat
 let as_nat h e =
   let s = as_seq h e in
   let s0 = s.[0] in
@@ -89,18 +24,8 @@ let as_nat h e =
   let s2 = s.[2] in
   let s3 = s.[3] in
   let s4 = s.[4] in
-  lemma_fits_as_nat5 (s0, s1, s2, s3, s4);
   S.as_nat5 (s0, s1, s2, s3, s4)
 
 noextract
-val fevalh: h:mem -> f:felem -> GTot P.elem
-let fevalh h f = (as_nat h f) % P.prime
-
-noextract
-val point_eval:h:mem -> p:point -> GTot Spec.Ed25519.ext_point
-let point_eval h p =
-  let x = gsub p 0ul 5ul in
-  let y = gsub p 5ul 5ul in
-  let z = gsub p 10ul 5ul in
-  let t = gsub p 15ul 5ul in
-  (fevalh h x, fevalh h y, fevalh h z, fevalh h t)
+val fevalh: h:mem -> f:felem -> GTot (n:nat{n < Spec.Ed25519.q})
+let fevalh h f = (as_nat h f) % Spec.Ed25519.q
