code/experimental/ed25519/Hacl.Impl.Load56.fst
@@ -9,7 +9,7 @@ open Lib.ByteSequence
 open Lib.Buffer
 open Lib.ByteBuffer
 
-module F = Hacl.Impl.Ed25519.Field56
+module F56 = Hacl.Impl.Ed25519.Field56
 
 val hload56_le:
     b:lbuffer uint8 64ul
@@ -61,7 +61,7 @@ val load_32_bytes:
   Stack unit
     (requires fun h -> live h out /\ live h b)
     (ensures  fun h0 _ h1 -> modifies (loc out) h0 h1 /\
-      F.as_nat h1 out == nat_from_bytes_le (as_seq h0 b)
+      F56.fevalh h1 out == nat_from_bytes_le (as_seq h0 b)
     )
 let load_32_bytes out b =
   let b0 = hload56_le' b 0ul in
