code/experimental/ed25519/Hacl.Impl.SHA512.ModQ.fst
@@ -8,7 +8,7 @@ open Lib.ByteSequence
 open Lib.Sequence
 open Lib.Buffer
 
-module F = Hacl.Impl.Ed25519.Field56
+module F56 = Hacl.Impl.Ed25519.Field56
 
 #reset-options "--max_fuel 0 --max_ifuel 0"
 
@@ -61,7 +61,7 @@ val sha512_modq_pre:
       live h input /\ live h out /\ live h prefix /\
       disjoint prefix out /\  disjoint out input)
     (ensures  fun h0 _ h1 -> modifies (loc out) h0 h1 /\
-      F.as_nat h1 out ==
+      F56.fevalh h1 out ==
       Spec.Ed25519.sha512_modq (32 + v len)
         (concat #uint8 #32 #(v len) (as_seq h0 prefix) (as_seq h0 input))
     )
@@ -89,7 +89,7 @@ val sha512_modq_pre_pre2:
       live h input /\ live h out /\ live h prefix /\ live h prefix2 /\
       disjoint prefix out /\ disjoint prefix2 out /\ disjoint out input)
     (ensures  fun h0 _ h1 ->  modifies (loc out) h0 h1 /\
-     F.as_nat h1 out ==
+     F56.fevalh h1 out ==
       Spec.Ed25519.sha512_modq (64 + v len)
         (concat #uint8 #64 #(v len)
           (concat #uint8 #32 #32
